Small cleanup of PreStar proofs

Lemke/FiniteAutomaton.thy
@@ -4,126 +4,131 @@ theory FiniteAutomaton
   imports "HOL-Data_Structures.Define_Time_Function"
 begin \<comment>\<open>begin-theory FiniteAutomaton\<close>
 
+subsection\<open>Definition\<close>
+
 record ('s, 't) nfa =
   transitions :: "('s \<times> 't \<times> 's) set"
   start :: 's
   finals :: "'s set"
 
-definition nfa_invar :: "('s, 't) nfa \<Rightarrow> bool" where
-  "nfa_invar M \<equiv> finite (transitions M)"
+subsection\<open>Step Relation\<close>
 
-fun step :: "('s \<times> 't \<times> 's) set \<Rightarrow> 't \<Rightarrow> 's \<Rightarrow> 's set" where
+definition step :: "('s \<times> 't \<times> 's) set \<Rightarrow> 't \<Rightarrow> 's \<Rightarrow> 's set" where
   "step T c s = { s' | s'. (s, c, s') \<in> T }"
 
-fun step' :: "('s \<times> 't \<times> 's) set \<Rightarrow> 't \<Rightarrow> 's set \<Rightarrow> 's set" where
-  "step' T c s = { s' | s'. \<exists>s\<^sub>0 \<in> s. s' \<in> step T c s\<^sub>0 }"
+definition Step :: "('s \<times> 't \<times> 's) set \<Rightarrow> 't \<Rightarrow> 's set \<Rightarrow> 's set" where
+  "Step T c s = { s' | s'. \<exists>s\<^sub>0 \<in> s. s' \<in> step T c s\<^sub>0 }"
 
-fun steps':: "('s \<times> 't \<times> 's) set \<Rightarrow> 't list \<Rightarrow> 's set \<Rightarrow> 's set" where
-  "steps' T w s = fold (step' T) w s"
+definition Steps :: "('s \<times> 't \<times> 's) set \<Rightarrow> 't list \<Rightarrow> 's set \<Rightarrow> 's set" where
+  "Steps T w s = fold (Step T) w s"
 
-fun steps :: "('s \<times> 't \<times> 's) set \<Rightarrow> 't list \<Rightarrow> 's \<Rightarrow> 's set" where
-  "steps T w s = steps' T w {s}"
+abbreviation steps :: "('s \<times> 't \<times> 's) set \<Rightarrow> 't list \<Rightarrow> 's \<Rightarrow> 's set" where
+  "steps T w s \<equiv> Steps T w {s}"
 
-lemma steps'_mono:
+lemma Steps_mono:
   assumes "s\<^sub>1 \<subseteq> s\<^sub>2"
-  shows "steps' T w s\<^sub>1 \<subseteq> steps' T w s\<^sub>2"
+  shows "Steps T w s\<^sub>1 \<subseteq> Steps T w s\<^sub>2"
 proof (insert assms; induction w arbitrary: s\<^sub>1 s\<^sub>2)
-  case Nil thus ?case by simp
+  case Nil thus ?case by (simp add: Steps_def)
 next
-  case (Cons a w)
-  then show ?case
-    by (smt (verit) fold_simps(2) mem_Collect_eq step'.simps steps'.simps subset_eq)
+  case (Cons w ws)
+
+  define s\<^sub>1' where [simp]: "s\<^sub>1' \<equiv> Step T w s\<^sub>1"
+  define s\<^sub>2' where [simp]: "s\<^sub>2' \<equiv> Step T w s\<^sub>2"
+  
+  have "s\<^sub>1' \<subseteq> s\<^sub>2'"
+    by (simp add: Step_def, use \<open>s\<^sub>1 \<subseteq> s\<^sub>2\<close> in blast)
+  then have "Steps T ws s\<^sub>1' \<subseteq> Steps T ws s\<^sub>2'"
+    by (elim Cons.IH)
+  moreover have "Steps T (w#ws) s\<^sub>1 = Steps T ws s\<^sub>1'"
+    by (simp add: Steps_def)
+  moreover have "Steps T (w#ws) s\<^sub>2 = Steps T ws s\<^sub>2'"
+    by (simp add: Steps_def)
+  ultimately show ?case
+    by simp
 qed
 
-lemma steps'_startExists:
-  assumes "q\<^sub>f \<in> steps' T w s"
+\<comment>\<open>Sanity check that a monotonicity rule is really defined:\<close>
+lemma [mono]: "mono (Steps T w)"
+  by (intro monoI, elim Steps_mono)
+
+lemma Steps_path:
+  assumes "q\<^sub>f \<in> Steps T w s"
   shows "\<exists>q\<^sub>0 \<in> s. q\<^sub>f \<in> steps T w q\<^sub>0"
 proof (insert assms; induction w arbitrary: s)
-  case Nil thus ?case by simp
+  case Nil thus ?case by (simp add: Steps_def)
 next
-  case (Cons a w)
-  then have "q\<^sub>f \<in> steps' T w (steps' T [a] s)"
-    by simp
-  then obtain q' where "q' \<in> steps' T [a] s" and "q\<^sub>f \<in> steps T w q'"
-    using Cons by blast
-  then have "q' \<in> step' T a s"
-    by simp
-  then obtain q\<^sub>0 where "q\<^sub>0 \<in> s" and "q' \<in> step T a q\<^sub>0"
-    by fastforce
-  then have "q' \<in> steps T [a] q\<^sub>0"
-    by simp
+  case (Cons w ws)
+  then have "q\<^sub>f \<in> Steps T ws (Step T w s)"
+    by (simp add: Steps_def)
+  moreover obtain q\<^sub>0 where "q\<^sub>0 \<in> (Step T w s)" and "q\<^sub>f \<in> steps T ws q\<^sub>0"
+    using Cons.IH calculation by blast
+  ultimately obtain q' where "q\<^sub>0 \<in> step T w q'" and "q' \<in> s"
+    unfolding Steps_def Step_def by blast
 
-  have "q\<^sub>f \<in> steps' T w (step T a q\<^sub>0)"
-    using \<open>q\<^sub>f \<in> steps T w q'\<close> \<open>q' \<in> step T a q\<^sub>0\<close>
-    by (metis (no_types, opaque_lifting) bot.extremum insert_subset steps'_mono steps.elims subset_eq)
-  then have "q\<^sub>f \<in> steps' T w (steps T [a] q\<^sub>0)"
-    by simp
-  then have "q\<^sub>f \<in> steps T (a#w) q\<^sub>0"
-    by simp
-  then show ?case
-    using \<open>q\<^sub>0 \<in> s\<close> by blast
+  note \<open>q\<^sub>0 \<in> step T w q'\<close> and \<open>q\<^sub>f \<in> steps T ws q\<^sub>0\<close>
+  then have "q\<^sub>f \<in> Steps T ws (step T w q')"
+    using Steps_mono[of "{q\<^sub>0}"] by blast
+  moreover have "Steps T ws (step T w q') = steps T (w#ws) q'"
+    by (simp add: Steps_def step_def Step_def)
+  ultimately show ?case
+    using \<open>q' \<in> s\<close> by blast
 qed
 
-lemma steps_split:
-  assumes "q\<^sub>f \<in> steps T (w\<^sub>1@w\<^sub>2) q\<^sub>0"
-  shows "\<exists>q'. q' \<in> steps T w\<^sub>1 q\<^sub>0 \<and> q\<^sub>f \<in> steps T w\<^sub>2 q'"
+lemma Steps_split:
+  assumes "q\<^sub>f \<in> Steps T (w\<^sub>1@w\<^sub>2) Q\<^sub>0"
+  shows "\<exists>q'. q' \<in> Steps T w\<^sub>1 Q\<^sub>0 \<and> q\<^sub>f \<in> steps T w\<^sub>2 q'"
 proof -
-  define s\<^sub>f where [simp add]: "s\<^sub>f = steps T (w\<^sub>1@w\<^sub>2) q\<^sub>0"
-  define s' where [simp add]: "s' = fold (step' T) w\<^sub>1 {q\<^sub>0}"
-
-  have "s\<^sub>f = fold (step' T) (w\<^sub>1@w\<^sub>2) {q\<^sub>0}"
-    by simp
-  then have "q\<^sub>f \<in> s\<^sub>f"
-    using assms by simp
-
-  have "s\<^sub>f = fold (step' T) w\<^sub>2 s'"
-    by simp
-  then have "s\<^sub>f = steps' T w\<^sub>2 s'"
-    by simp
-  then obtain q' where "q' \<in> s'" and "q\<^sub>f \<in> steps T w\<^sub>2 q'"
-    using steps'_startExists assms by fastforce
-  moreover have "q' \<in> steps T w\<^sub>1 q\<^sub>0"
+  define Q\<^sub>f where [simp]: "Q\<^sub>f = Steps T (w\<^sub>1@w\<^sub>2) Q\<^sub>0"
+  define Q' where [simp]: "Q' = Steps T w\<^sub>1 Q\<^sub>0"
+  have "Q\<^sub>f = Steps T w\<^sub>2 Q'"
+    by (simp add: Steps_def)
+  then obtain q' where "q' \<in> Q'" and "q\<^sub>f \<in> steps T w\<^sub>2 q'"
+    using assms Steps_path by force
+  moreover have "q' \<in> Steps T w\<^sub>1 Q\<^sub>0"
     using calculation by simp
   ultimately show ?thesis
     by blast
 qed
 
-lemma steps_split3:
-  assumes "q\<^sub>f \<in> steps T (w\<^sub>1@w\<^sub>2@w\<^sub>3) q\<^sub>0"
-  shows "\<exists>q' q''. q' \<in> steps T w\<^sub>1 q\<^sub>0 \<and> q'' \<in> steps T w\<^sub>2 q' \<and> q\<^sub>f \<in> steps T w\<^sub>3 q''"
-  using assms steps_split by metis
-
-lemma steps_join:
-  assumes "q' \<in> steps T w\<^sub>1 q\<^sub>0" and "q\<^sub>f \<in> steps T w\<^sub>2 q'"
-  shows "q\<^sub>f \<in> steps T (w\<^sub>1@w\<^sub>2) q\<^sub>0"
+lemma Steps_join:
+  assumes "q' \<in> Steps T w\<^sub>1 Q\<^sub>0" and "q\<^sub>f \<in> steps T w\<^sub>2 q'"
+  shows "q\<^sub>f \<in> Steps T (w\<^sub>1@w\<^sub>2) Q\<^sub>0"
 proof -
-  define s' where [simp add]: "s' = steps T w\<^sub>1 q\<^sub>0"
-  define s\<^sub>f where [simp add]: "s\<^sub>f = steps' T w\<^sub>2 s'"
+  define Q' where [simp]: "Q' = Steps T w\<^sub>1 Q\<^sub>0"
+  define Q\<^sub>f where [simp]: "Q\<^sub>f = Steps T w\<^sub>2 Q'"
 
-  have "{q'} \<subseteq> s'"
+  have "{q'} \<subseteq> Q'"
     using assms(1) by simp
-  then have "steps' T w\<^sub>2 {q'} \<subseteq> steps' T w\<^sub>2 s'"
-    using steps'_mono by blast
-  then have "q\<^sub>f \<in> steps' T w\<^sub>2 s'"
+  then have "Steps T w\<^sub>2 {q'} \<subseteq> Steps T w\<^sub>2 Q'"
+    using Steps_mono by blast
+  then have "q\<^sub>f \<in> Steps T w\<^sub>2 Q'"
     using assms(2) by fastforce
-  moreover have "s\<^sub>f = steps T (w\<^sub>1@w\<^sub>2) q\<^sub>0"
-    by simp
+  moreover have "Q\<^sub>f = Steps T (w\<^sub>1@w\<^sub>2) Q\<^sub>0"
+    by (simp add: Steps_def)
   ultimately show ?thesis
     by simp
 qed
 
-lemma steps_join3:
+lemma Steps_split3:
+  assumes "q\<^sub>f \<in> Steps T (w\<^sub>1@w\<^sub>2@w\<^sub>3) Q\<^sub>0"
+  shows "\<exists>q' q''. q' \<in> Steps T w\<^sub>1 Q\<^sub>0 \<and> q'' \<in> steps T w\<^sub>2 q' \<and> q\<^sub>f \<in> steps T w\<^sub>3 q''"
+  using assms Steps_split by meson
+
+lemma Steps_join3:
   assumes "q' \<in> steps T w\<^sub>1 q\<^sub>0" and "q'' \<in> steps T w\<^sub>2 q'" and "q\<^sub>f \<in> steps T w\<^sub>3 q''"
   shows "q\<^sub>f \<in> steps T (w\<^sub>1@w\<^sub>2@w\<^sub>3) q\<^sub>0"
-  using assms steps_join by metis
+  using assms Steps_join by metis
 
-definition accepts :: "('s \<times> 't \<times> 's) set \<Rightarrow> 's \<Rightarrow> 's set \<Rightarrow> 't list \<Rightarrow> bool" where
-  "accepts T S F w \<equiv> (steps T w S \<inter> F \<noteq> {})"
+subsection\<open>Language\<close>
+
+abbreviation accepts :: "('s \<times> 't \<times> 's) set \<Rightarrow> 's \<Rightarrow> 's set \<Rightarrow> 't list \<Rightarrow> bool" where
+  "accepts T s F w \<equiv> (steps T w s \<inter> F \<noteq> {})"
 
 lemma accepts_split3:
-  assumes "accepts T S F (w\<^sub>1@w\<^sub>2@w\<^sub>3)"
-  shows "\<exists>q' q'' q\<^sub>f. q' \<in> steps T w\<^sub>1 S \<and> q'' \<in> steps T w\<^sub>2 q' \<and> q\<^sub>f \<in> steps T w\<^sub>3 q'' \<and> q\<^sub>f \<in> F"
-  using assms steps_split3 accepts_def by (metis Int_emptyI)
+  assumes "accepts T s F (w\<^sub>1@w\<^sub>2@w\<^sub>3)"
+  shows "\<exists>q' q'' q\<^sub>f. q' \<in> steps T w\<^sub>1 s \<and> q'' \<in> steps T w\<^sub>2 q' \<and> q\<^sub>f \<in> steps T w\<^sub>3 q'' \<and> q\<^sub>f \<in> F"
+  using assms Steps_split3 by fast
 
 definition lang' :: "('s \<times> 't \<times> 's) set \<Rightarrow> 's \<Rightarrow> 's set \<Rightarrow> ('t list) set" where
   "lang' T S F \<equiv> { w | w. accepts T S F w }"
@@ -136,11 +141,11 @@ lemma nfa_lang_trans:
   shows "(w\<^sub>1@w\<^sub>2) \<in> lang' T s F"
 proof -
   obtain q\<^sub>f where "q\<^sub>f \<in> steps T w\<^sub>2 s'" and "q\<^sub>f \<in> F"
-    using assms(2) unfolding lang'_def accepts_def by blast
+    using assms(2) unfolding lang'_def by blast
   moreover have "q\<^sub>f \<in> steps T (w\<^sub>1@w\<^sub>2) s"
-    using assms(1) \<open>q\<^sub>f \<in> steps T w\<^sub>2 s'\<close> by (rule steps_join)
+    using assms(1) \<open>q\<^sub>f \<in> steps T w\<^sub>2 s'\<close> by (rule Steps_join)
   ultimately show ?thesis
-    unfolding lang'_def accepts_def using \<open>q\<^sub>f \<in> F\<close> by blast
+    unfolding lang'_def using \<open>q\<^sub>f \<in> F\<close> by blast
 qed
 
 lemma nfa_lang_split:
@@ -148,11 +153,11 @@ lemma nfa_lang_split:
   obtains q' where "q' \<in> steps T w\<^sub>1 q" and "w\<^sub>2 \<in> lang' T q' F"
 proof -
   obtain q\<^sub>f where "q\<^sub>f \<in> steps T (w\<^sub>1@w\<^sub>2) q" and "q\<^sub>f \<in> F"
-    using assms unfolding lang'_def accepts_def by blast
+    using assms unfolding lang'_def by blast
   then obtain q' where "q' \<in> steps T w\<^sub>1 q" and "q\<^sub>f \<in> steps T w\<^sub>2 q'"
-    using steps_split by fast
+    using Steps_split by fast
   moreover have "w\<^sub>2 \<in> lang' T q' F"
-    unfolding lang'_def accepts_def using \<open>q\<^sub>f \<in> F\<close> calculation by blast
+    unfolding lang'_def using \<open>q\<^sub>f \<in> F\<close> calculation by blast
   ultimately show ?thesis
     using that by blast
 qed
